MathematicalLogic.lean
@@ -1,5 +1,6 @@
 import MathematicalLogic.Notation
 import MathematicalLogic.Vector
+import MathematicalLogic.ZFSet
 
 import MathematicalLogic.FirstOrder.Syntax
 import MathematicalLogic.FirstOrder.Semantics
@@ -11,10 +12,10 @@ import MathematicalLogic.FirstOrder.Completeness.Lindenbaum
 import MathematicalLogic.FirstOrder.Completeness.TermModel
 import MathematicalLogic.FirstOrder.Completeness.Completeness
 import MathematicalLogic.FirstOrder.Encoding
+import MathematicalLogic.FirstOrder.Arithmetic.Theory
 
 import MathematicalLogic.SecondOrder.Syntax
 import MathematicalLogic.SecondOrder.Semantics
 import MathematicalLogic.SecondOrder.Peano
 import MathematicalLogic.SecondOrder.Real
-import MathematicalLogic.ZFSet
 import MathematicalLogic.SecondOrder.ZF
